# Examples:
- ![[Advanced Math Example 1.png]]`When a polynomial is divided by a binomial, you can plug in that factor into the polynomial. So, for this question, you can plug in 1 into the equation and it should equal -1 as that's the remainder.` $c^2(1)^4 +4c(1)^2-6 = -1$ `After simplifying you are left with` $c^2 + 4c -5 = 0$ `Apply the quadratic equation to get the two roots` $\frac {-4 + \sqrt{36}} {2} = 1$ `and` $\frac {-4 - \sqrt {36}} {2} = -5$ `Since the question states that c > 0, then c must be 1.`

- ![[Advanced Math Example 2.png]]
	`For this question, vertex form would be the best form to use.` $y=a(x-h)^2+k$ `Since the vertex in this problem is given as (8,-1), the equation can be written as` $y=a(x-8)^2 -1$ `Given this equation the value of the root can be plugged in (15, 0), giving us` $0 = a(15-8)^2 -1$ `Which simplifies down to` $1 = 49a$ `and therefore` $a = \frac 1 {49}$  `The overall equaiton is now` $y = \frac 1 {49}(x-8)^2 -1$ `To find the y-intercept of the parabola, plug 0 in for x` $y = \frac 1 {49} (0-8)^2 -1$ `This simplifies to` $y = \frac 1 {49}(64) - 1$ `This then becomes` $y=\frac {64} {49} - 1$ `Which gives us our y-intercept of` $y=\frac {15} {49}$


